theories/set.v
@@ -1,0 +1,37 @@
+Require Import minilog.operators.
+
+(** * Operations over sets *)
+
+Section Pset.
+
+Variable A : Type.
+
+Definition pset := (A -> Prop).
+
+Definition inter (P Q : pset) : pset :=
+  fun x => P x /\ Q x.
+
+Definition union (P Q : pset) : pset :=
+  fun x => P x \/ Q x.
+
+Definition diff (P Q : pset) : pset :=
+  fun x => P x /\ ~Q x.
+
+Definition comp (P : pset) : pset :=
+  fun x => ~P x.
+
+Definition subseteq (P Q : pset) :=
+  forall x, P x -> Q x.
+
+Definition subset (P Q : pset) :=
+  subseteq P Q /\ exists x, Q x /\ ~Q x.
+
+Definition emptyset : pset := fun _ => False.
+
+End Pset.
+
+Instance inter_cap (A : Type) : CapOp (pset A) := inter A.
+Instance union_cup (A : Type) : CupOp (pset A) := union A.
+Instance subseteq_subseteq (A : Type) : SubseteqOp (pset A) := subseteq A.
+Instance subset_subset (A : Type) : SubsetOp (pset A) := subset A.
+Notation "∅" := (emptyset _).
