theories/operators.v
@@ -1,0 +1,27 @@
+Declare Scope ops.
+Delimit Scope ops with ops.
+
+Class InOp (x X : Type) :=
+  in_op_ : x -> X -> Prop.
+
+Notation "x ∈ X" := (in_op_ x X) (at level 39) : ops.
+
+Class CupOp (A : Type) :=
+  cup_op_ : A -> A -> A.
+
+Notation "x ∪ y" := (cup_op_ x y) (at level 40) : ops.
+
+Class CapOp (A : Type) :=
+  cap_op_ : A -> A -> A.
+
+Notation "x ∩ y" := (cap_op_ x y) (at level 40) : ops.
+
+Class SubsetOp (A : Type) :=
+  subset_op_ : A -> A -> Prop.
+
+Notation "x ⊂ y" := (subset_op_ x y) (at level 39) : ops.
+
+Class SubseteqOp (A : Type) :=
+  subseteq_op_ : A -> A -> Prop.
+
+Notation "x ⊆ y" := (subseteq_op_ x y) (at level 39) : ops.
